language_formal/spark2014_semantics/test.v
@@ -1,0 +1,191 @@
+Require Import semantics.
+Require Import wellformedness.
+
+(****************
+  - Example 1 -
+ ****************)
+
+(* = = = = = = = = = = = = = =
+  procedure Test_for_Coq
+  is 
+     N: Integer := 25;
+     Result: Boolean;
+     I: Integer;
+     X: Integer;
+  begin
+     Result := true;
+     if N <= 1 then
+        Result := false;
+     end if;
+     I := 2;
+     while I*I <= N loop
+        X := N / I;
+        if N = X * I then
+           Result := false;
+        end if;
+        I := I + 1;
+     end loop;
+  end Test_for_Coq;
+ = = = = = = = = = = = = = =*)
+
+Definition f_prime :=
+(* Procedure Body Declaration *)
+      Sproc 3 (
+        mkprocedure_body 4
+          (* Procedure Body - Name *)
+          (*Test_for_Coq*) 1
+          (* Procedure Body - Specification *)
+          (nil)
+          (* Procedure Body - Parameters *)
+          (nil) 
+          (* Procedure Body - Locally Defined Variables *)
+          (
+          mklocal_declaration 5 (*N*) 1 1 (Some (Econst 6 (Ointconst 25))) :: 
+          mklocal_declaration 7 (*Result*) 2 2 None :: 
+          mklocal_declaration 8 (*I*) 3 1 None :: 
+          mklocal_declaration 9 (*X*) 4 1 None :: nil)
+          (* Procedure Body - Body *) (
+            Sseq 10 (
+              Sassign 11 ((*Result*) 2) (Econst 12 (Oboolconst true)) ) ( 
+              Sseq 13 (
+                Sifthen 14 (Ebinop 15 Cle (Evar 16 (*N*) 1) (Econst 17 (Ointconst 1))) (
+                    Sassign 18 ((*Result*) 2) (Econst 19 (Oboolconst false))
+                  ) ) ( 
+                Sseq 20 (
+                  Sassign 21 ((*I*) 3) (Econst 22 (Ointconst 2)) ) ( 
+                  Swhile 23 (Ebinop 24 Cle (Ebinop 25 Omul (Evar 26 (*I*) 3) (Evar 27 (*I*) 3)) (Evar 28 (*N*) 1)) (
+                      Sseq 29 (
+                        Sassign 30 ((*X*) 4) (Ebinop 31 Odiv (Evar 32 (*N*) 1) (Evar 33 (*I*) 3)) ) ( 
+                        Sseq 34 (
+                          Sifthen 35 (Ebinop 36 Ceq (Evar 37 (*N*) 1) (Ebinop 38 Omul (Evar 39 (*X*) 4) (Evar 40 (*I*) 3))) (
+                              Sassign 41 ((*Result*) 2) (Econst 42 (Oboolconst false))
+                            ) ) ( 
+                          Sassign 43 ((*I*) 3) (Ebinop 44 Oadd (Evar 45 (*I*) 3) (Econst 46 (Ointconst 1))) ) )
+                    ) ) ) )
+          )
+      ).
+
+Check f_prime.
+
+Definition result := f_eval_subprogram 100 nil f_prime.
+
+Eval compute in result.
+
+Definition ast_num_inc := f_ast_num_inc_subprogram f_prime.
+
+Eval compute in ast_num_inc.
+
+Definition well_typed := f_well_typed_subprogram nil f_prime.
+
+Eval compute in well_typed.
+
+Definition well_initialized := f_well_defined_subprogram nil f_prime.
+
+Eval compute in well_initialized.
+
+Definition well_checked := f_check_generator_subprogram nil f_prime.
+
+Eval compute in well_checked.
+
+Definition run_time_checks := well_checked.
+
+Definition result_with_checks := f_eval_subprogram_with_checks 100 run_time_checks nil f_prime.
+
+Eval compute in result_with_checks.
+
+
+
+(****************
+  - Example 2 -
+ ****************)
+
+(* = = = = = = = = = = = = = =
+  procedure Test_for_Coq1
+  is 
+     N: Integer := 25;
+     Result: Boolean;
+     I: Integer;
+     X: Integer;
+  begin
+     Result := true;
+     if N <= 1 then
+        Result := false;
+     end if;
+     I := 0;
+     while I*I <= N loop
+        X := N / I;
+        if N = X * I then
+           Result := false;
+        end if;
+        I := I + 1;
+     end loop;
+  end Test_for_Coq1;
+ = = = = = = = = = = = = = =*)
+
+Definition f_prime_div_zero :=
+(* Procedure Body Declaration *)
+      Sproc 3 (
+        mkprocedure_body 4
+          (* Procedure Body - Name *)
+          (*Test_for_Coq1*) 1
+          (* Procedure Body - Specification *)
+          (nil)
+          (* Procedure Body - Parameters *)
+          (nil) 
+          (* Procedure Body - Locally Defined Variables *)
+          (
+          mklocal_declaration 5 (*N*) 1 2 (Some (Econst 6 (Ointconst 25))) :: 
+          mklocal_declaration 7 (*Result*) 2 3 None :: 
+          mklocal_declaration 8 (*I*) 3 2 None :: 
+          mklocal_declaration 9 (*X*) 4 2 None :: nil)
+          (* Procedure Body - Body *) (
+            Sseq 10 (
+              Sassign 11 ((*Result*) 2) (Econst 12 (Oboolconst true)) ) ( 
+              Sseq 13 (
+                Sifthen 14 (Ebinop 15 Cle (Evar 16 (*N*) 1) (Econst 17 (Ointconst 1))) (
+                    Sassign 18 ((*Result*) 2) (Econst 19 (Oboolconst false))
+                  ) ) ( 
+                Sseq 20 (
+                  Sassign 21 ((*I*) 3) (Econst 22 (Ointconst 0)) ) ( 
+                  Swhile 23 (Ebinop 24 Cle (Ebinop 25 Omul (Evar 26 (*I*) 3) (Evar 27 (*I*) 3)) (Evar 28 (*N*) 1)) (
+                      Sseq 29 (
+                        Sassign 30 ((*X*) 4) (Ebinop 31 Odiv (Evar 32 (*N*) 1) (Evar 33 (*I*) 3)) ) ( 
+                        Sseq 34 (
+                          Sifthen 35 (Ebinop 36 Ceq (Evar 37 (*N*) 1) (Ebinop 38 Omul (Evar 39 (*X*) 4) (Evar 40 (*I*) 3))) (
+                              Sassign 41 ((*Result*) 2) (Econst 42 (Oboolconst false))
+                            ) ) ( 
+                          Sassign 43 ((*I*) 3) (Ebinop 44 Oadd (Evar 45 (*I*) 3) (Econst 46 (Ointconst 1))) ) )
+                    ) ) ) )
+          )
+      ).
+
+Definition result_1 := f_eval_subprogram 100 nil f_prime_div_zero.
+
+Eval compute in result_1.
+
+Definition run_time_checks_1 := f_check_generator_subprogram nil f_prime.
+
+Eval compute in run_time_checks_1.
+
+Definition result_with_checks_1 := f_eval_subprogram_with_checks 100 run_time_checks_1 nil f_prime_div_zero.
+
+Eval compute in result_with_checks_1.
+
+Definition result_without_checks_1 := f_eval_subprogram_with_checks 100 nil nil f_prime_div_zero.
+
+Eval compute in result_without_checks_1.
+
+Definition ast_num_inc_1 := f_ast_num_inc_subprogram f_prime_div_zero.
+
+Eval compute in ast_num_inc_1.
+
+
+(* ======================================================== *)
+(* ======================================================== *)
+
+
+
+
+
+
+
